WIP

code/ecdsa/dist/Hacl_P256.c
@@ -2017,38 +2017,9 @@ static void mul_atomic(uint64_t x, uint64_t y, uint64_t *result, uint64_t *temp)
   temp[0U] = h0;
 }
 
-static void montgomery_multiplication_round_(Spec_P256_curve c, uint64_t *t, uint64_t *t2)
+static void montgomery_multiplication_round_w_k0(Spec_P256_curve c, uint64_t *t, uint64_t *t2)
 {
   uint64_t t1 = t[0U];
-  uint64_t t1_buffer = t1;
-  const uint64_t *primeBuffer;
-  switch (c)
-  {
-    case Spec_P256_P256:
-      {
-        primeBuffer = prime256_buffer;
-        break;
-      }
-    case Spec_P256_P384:
-      {
-        primeBuffer = prime384_buffer;
-        break;
-      }
-    default:
-      {
-        KRML_HOST_EPRINTF("KreMLin incomplete match at %s:%d\n", __FILE__, __LINE__);
-        KRML_HOST_EXIT(253U);
-      }
-  }
-  uint64_t primeBuffer0 = primeBuffer[0U];
-  uint64_t temp;
-  if (!(primeBuffer0 == (uint64_t)0xffffffffffffffffU))
-  {
-    temp = (uint64_t)0U;
-    uint64_t k0 = getK0(c);
-    mul_atomic(t1, k0, &t1_buffer, &temp);
-  }
-  uint64_t t11 = t1_buffer;
   const uint64_t *sw;
   switch (c)
   {
@@ -2068,7 +2039,67 @@ static void montgomery_multiplication_round_(Spec_P256_curve c, uint64_t *t, uin
         KRML_HOST_EXIT(253U);
       }
   }
-  short_mul_bn(c, sw, t11, t2);
+  short_mul_bn(c, sw, t1, t2);
+}
+
+static void
+montgomery_multiplication_round_k0(Spec_P256_curve c, uint64_t k0, uint64_t *t, uint64_t *t2)
+{
+  uint64_t t1 = t[0U];
+  uint64_t y = (uint64_t)0U;
+  uint64_t temp = (uint64_t)0U;
+  mul_atomic(t1, k0, &y, &temp);
+  uint64_t y_ = y;
+  const uint64_t *sw;
+  switch (c)
+  {
+    case Spec_P256_P256:
+      {
+        sw = prime256_buffer;
+        break;
+      }
+    case Spec_P256_P384:
+      {
+        sw = prime384_buffer;
+        break;
+      }
+    default:
+      {
+        KRML_HOST_EPRINTF("KreMLin incomplete match at %s:%d\n", __FILE__, __LINE__);
+        KRML_HOST_EXIT(253U);
+      }
+  }
+  short_mul_bn(c, sw, y_, t2);
+}
+
+static void montgomery_multiplication_round_(Spec_P256_curve c, uint64_t *t, uint64_t *t2)
+{
+  uint64_t sw;
+  switch (c)
+  {
+    case Spec_P256_P256:
+      {
+        sw = (uint64_t)0xffffffffffffffffU;
+        break;
+      }
+    case Spec_P256_P384:
+      {
+        sw = (uint64_t)0xffffffffU;
+        break;
+      }
+    default:
+      {
+        KRML_HOST_EPRINTF("KreMLin incomplete match at %s:%d\n", __FILE__, __LINE__);
+        KRML_HOST_EXIT(253U);
+      }
+  }
+  if (sw == (uint64_t)0xffffffffffffffffU)
+  {
+    montgomery_multiplication_round_w_k0(c, t, t2);
+    return;
+  }
+  uint64_t k0 = getK0(c);
+  montgomery_multiplication_round_k0(c, k0, t, t2);
 }
 
 static void montgomery_multiplication_round(Spec_P256_curve c, uint64_t *t, uint64_t *round)
